Reflection/Derive.lean
@@ -1,0 +1,73 @@
+import Lean
+import Reflection.MutualInductive
+import Qq
+
+open Lean Meta Elab Term Qq
+
+#check InductiveVal
+
+private partial def getTyₛ (tys : Expr) : MetaM Q(Tyₛ.{u}) := do
+  forallBoundedTelescope tys (some 1) fun var body => do
+    if var.isEmpty then
+      return q(Tyₛ.U.{u})
+    else
+      let var := var[0]!
+      let ty : Q(Type u) <- var.fvarId!.getType
+      let rest : Q(Tyₛ.{u}) <- getTyₛ body -- rest is for example `var : X ⊢ SPi ...`
+      let rest : Q($ty -> Tyₛ.{u}) <- mkLambdaFVars #[var] rest
+      return q(Tyₛ.SPi.{u} $ty $rest)
+
+-- def skipParams (nParams : Nat) (e : Expr) : MetaM Expr := do
+--   forallBoundedTelescope
+
+elab "%Tyₛ " t:term : term => do
+  let t <- elabTermAndSynthesize t none
+  let u <- mkFreshLevelMVar
+  getTyₛ (u:=u) t
+-- elab "%Tyₛ " i:ident : term => do
+--   let ind <- getConstInfoInduct i.getId
+--   let u <- mkFreshLevelMVar
+--   getTyₛ (u:=u) ind.type
+
+#check Nat
+
+#check %Tyₛ (Nat -> Type)
+
+/-- Given a `T` such as `Vec 123 : Type`, produce `Tmₛ.app (Tmₛ.var Varₛ.vz) 123 : Tmₛ _ Tyₛ.U`.
+  Given `Vec : Nat -> Type`, produce `Tmₛ.var Varₛ.vz : Tmₛ _ (Tyₛ.SPi Nat fun _ => Tyₛ.U)`. -/
+private partial def getTmₛ (Γₛ : Q(Conₛ.{u})) (Aₛ : Q(Tyₛ.{u})) (T : Expr) : MetaM Q(Tmₛ.{u} $Γₛ $Aₛ) := do
+  match <- Meta.whnf T with
+  | .app t u =>
+    let t := t
+    let tt <- getTmₛ Γₛ Aₛ t
+    q(Tmₛ.app )
+  | .fvar _ => q(Tmₛ.var Varₛ.vz)
+  | _ => throwError "uh oh"
+
+elab "%Tmₛ " T:term : term => do
+  let T <- elabTerm T none
+  -- let  := T.getAppFn
+  let ind <- getConstInfoInduct (getAppFn)
+  getTyₚ ind.type
+
+private partial def getTyₚ (Γₛ : Q(Conₛ.{u})) (args : Expr) : MetaM Q(Tyₚ.{u} $Γₛ) := do
+  forallBoundedTelescope args (some 1) fun var body => do
+    let u <- mkFreshLevelMVar
+    if var.isEmpty then
+      -- body is e.g. `Vec 123`.
+      let T <- getTmₛ Γₛ q(Tyₛ.U) body
+      return q(Tyₚ.El $(T))
+    else
+      let var := var[0]!
+      let ty : Q(Type u) <- var.fvarId!.getType
+      let rest : Expr <- getTyₛ body -- rest is for example `var : X ⊢ SPi ...`
+      let rest : Q($ty -> Tyₛ.{u}) <- mkLambdaFVars #[var] rest -- rest is for example `⊢ fun var:X => SPi ...`
+      return q(Tyₛ.SPi.{u} $ty $rest)
+
+
+elab "%Tyₚ " i:ident : term => do
+  let ind <- getConstInfoInduct i.getId
+  getTyₚ ind.type
+
+#check Vec
+#check %Tyₛ Vec
