Reflection/Util/EqHelpers.lean
@@ -7,3 +7,7 @@ theorem eq_cast_trans  (h₁ : A = B) (h₂ : B = C) (x : A)
 theorem eq_symm_cancel {T : I -> Type u} {a b : I} (h : a = b) (x : T b)
   : h ▸ h.symm ▸ x = x
   := by cases h; rfl
+
+/-- Universe-polymorphic version of `forall_congr`. Thanks Arthur! -/
+theorem forall_pcongr {α : Sort u} {p q : α → Sort v} (h : ∀ a, p a = q a) : (∀ a, p a) = (∀ a, q a) :=
+  (funext h : p = q) ▸ rfl
