lakefile.lean
@@ -5,9 +5,10 @@ package «reflection» {
   -- add package configuration options here
 }
 
--- require aesop from git "https://github.com/leanprover-community/aesop" -- 01cb707de69cf88733addfff0bacc710efae8d20
-require std from git "https://github.com/leanprover/std4" @ "v4.5.0-rc1"
-require aesop from git "https://github.com/JLimperg/aesop" @ "v4.5.0-rc1"
+require std from git "https://github.com/leanprover/std4" @ "v4.6.0-rc1"
+require aesop from git "https://github.com/JLimperg/aesop" @ "v4.6.0-rc1"
+-- require IIT from git "https://github.com/arthur-adjedj/iit" @ "v4.4.0"
+require Qq from git "https://github.com/leanprover-community/quote4"
 
 @[default_target]
 lean_lib «Reflection» {
